This file defines some extras properties needed for the TBR development.  After
the development, the proofs should be disseminated into the relevant files.

```agda

{-# OPTIONS --allow-unsolved-metas --exact-split --auto-inline --without-K
            --lossy-unification #-}

module TBR.DyadicExtras where

open import MLTT.Spartan renaming (_+_ to _‚àî_)
open import Naturals.Addition renaming (_+_ to _‚Ñï+_)
open import Naturals.Exponentiation
open import Naturals.Multiplication renaming (_*_ to _‚Ñï*_)
open import Naturals.Properties
open import Integers.Exponentiation
open import Integers.Multiplication renaming (_*_ to _‚Ñ§*_)
open import Integers.Order
open import Integers.Type
open import Integers.Addition renaming (_-_ to _‚Ñ§-_ ; _+_ to _‚Ñ§+_)
open import Integers.Negation renaming (-_ to ‚Ñ§-_)
open import Dyadics.Addition
open import Dyadics.Multiplication
open import Dyadics.Negation
open import Dyadics.Type
open import Dyadics.Order
open import Notation.Order
open import UF.Base

‚Ñ§[1/2]-is-positive : ‚Ñ§[1/2] ‚Üí ùì§‚ÇÄ Ãá
‚Ñ§[1/2]-is-positive p = 0‚Ñ§[1/2] < p

‚Ñ§[1/2]<-neg : (x y : ‚Ñ§[1/2]) ‚Üí 0‚Ñ§[1/2] < y ‚Üí x - y < x
‚Ñ§[1/2]<-neg x y l = Œ≥
 where
  I : - y < 0‚Ñ§[1/2]
  I = ‚Ñ§[1/2]<-swap 0‚Ñ§[1/2] y l

  II : x - y < x - 0‚Ñ§[1/2]
  II = ‚Ñ§[1/2]<-addition-preserves-order' (- y) 0‚Ñ§[1/2] x I

  III : x - 0‚Ñ§[1/2] Ôºù x
  III = x - 0‚Ñ§[1/2] Ôºù‚ü® refl                        ‚ü©
        x + 0‚Ñ§[1/2] Ôºù‚ü® ‚Ñ§[1/2]-zero-right-neutral x ‚ü©
        x           ‚àé

  Œ≥ : x - y < x
  Œ≥ = transport (x - y <_) III II

‚Ñ§[1/2]-0<1 : 0‚Ñ§[1/2] < 1‚Ñ§[1/2]
‚Ñ§[1/2]-0<1 = 0 , refl

‚Ñ§[1/2]<-1/2 : (x : ‚Ñ§[1/2]) ‚Üí 0‚Ñ§[1/2] < x ‚Üí 0‚Ñ§[1/2] < 1/2‚Ñ§[1/2] * x
‚Ñ§[1/2]<-1/2 x l = Œ≥
 where
  Œ≥ : 0‚Ñ§[1/2] < 1/2‚Ñ§[1/2] * x
  Œ≥ = ‚Ñ§[1/2]<-pos-multiplication-preserves-order 1/2‚Ñ§[1/2] x ‚Ñ§[1/2]-0<1/2 l

‚Ñ§[1/2]-trichotomous : (p q : ‚Ñ§[1/2]) ‚Üí (p < q) ‚àî (p Ôºù q) ‚àî (q < p)
‚Ñ§[1/2]-trichotomous ((p , a) , Œ±) ((q , b) , Œ≤) = Œ≥ I
 where
  I : trich-locate (p ‚Ñ§* pos (2^ b)) (q ‚Ñ§* pos (2^ a))
  I = ‚Ñ§-trichotomous (p ‚Ñ§* pos (2^ b)) (q ‚Ñ§* pos (2^ a))
  
  Œ≥ : trich-locate (p ‚Ñ§* pos (2^ b)) (q ‚Ñ§* pos (2^ a))
    ‚Üí ((p , a) , Œ±) < ((q , b) , Œ≤)
    ‚àî (((p , a) , Œ±) Ôºù ((q , b) , Œ≤))
    ‚àî (((q , b) , Œ≤) < (((p , a) , Œ±)))
  Œ≥ (inl l)       = inl l
  Œ≥ (inr (inr l)) = inr (inr l)
  Œ≥ (inr (inl e)) = inr (inl Œ≥')
   where
    Œ≥' : (p , a) , Œ± Ôºù (q , b) , Œ≤
    Œ≥' = ‚âà-to-Ôºù ((p , a) , Œ±) ((q , b) , Œ≤) e

‚Ñ§[1/2]<-addition-cancellable : (a b c : ‚Ñ§[1/2])
                             ‚Üí a + b < c + b
                             ‚Üí a < c
‚Ñ§[1/2]<-addition-cancellable a b c l = Œ≥
 where
  I : a + b - b < c + b - b
  I = ‚Ñ§[1/2]<-addition-preserves-order (a + b) (c + b) (- b) l

  II : (u v : ‚Ñ§[1/2]) ‚Üí u + v - v Ôºù u
  II u v = u + v - v   Ôºù‚ü® ‚Ñ§[1/2]+-assoc u v (- v)                   ‚ü©
           u + (v - v) Ôºù‚ü® ap (u +_) (‚Ñ§[1/2]+-inverse-sum-to-zero v) ‚ü©
           u + 0‚Ñ§[1/2] Ôºù‚ü® ‚Ñ§[1/2]-zero-right-neutral u               ‚ü© 
           u           ‚àé

  III : a + b - b Ôºù a
  III = II a b

  IV : c + b - b Ôºù c
  IV = II c b

  Œ≥ : a < c
  Œ≥ = transport‚ÇÇ _<_ III IV I

‚Ñ§[1/2]<-addition-cancellable' : (a b c : ‚Ñ§[1/2])
                              ‚Üí b + a < b + c
                              ‚Üí a < c
‚Ñ§[1/2]<-addition-cancellable' a b c l = Œ≥
 where
  I : b + a Ôºù a + b
  I = ‚Ñ§[1/2]+-comm b a

  II : b + c Ôºù c + b
  II = ‚Ñ§[1/2]+-comm b c

  III : a + b < c + b
  III = transport‚ÇÇ _<_ I II l

  Œ≥ : a < c
  Œ≥ = ‚Ñ§[1/2]<-addition-cancellable a b c III

‚Ñ§[1/2]<-adding : (a b c d : ‚Ñ§[1/2])
               ‚Üí a < b
               ‚Üí c < d
               ‚Üí a + c < b + d
‚Ñ§[1/2]<-adding a b c d l‚ÇÅ l‚ÇÇ = Œ≥
 where
  I : a + c < b + c
  I = ‚Ñ§[1/2]<-addition-preserves-order a b c l‚ÇÅ

  II : b + c < b + d
  II = ‚Ñ§[1/2]<-addition-preserves-order' c d b l‚ÇÇ

  Œ≥ : a + c < b + d
  Œ≥ = ‚Ñ§[1/2]<-trans (a + c) (b + c) (b + d) I II

‚Ñ§[1/2]<-swap' : (p q : ‚Ñ§[1/2]) ‚Üí - p < - q ‚Üí q < p
‚Ñ§[1/2]<-swap' p q l = Œ≥
 where
  I : - (- q) < - (- p)
  I = ‚Ñ§[1/2]<-swap (- p) (- q) l

  II : - (- q) Ôºù q
  II = ‚Ñ§[1/2]-minus-minus q ‚Åª¬π

  III : - (- p) Ôºù p
  III = ‚Ñ§[1/2]-minus-minus p ‚Åª¬π

  Œ≥ : q < p
  Œ≥ = transport‚ÇÇ _<_ II III I

‚Ñ§[1/2]-ordering-property : (a b c d : ‚Ñ§[1/2])
                         ‚Üí (a - b) < (c - d)
                         ‚Üí (a < c) ‚àî (d < b)
‚Ñ§[1/2]-ordering-property a b c d l‚ÇÅ = Cases (‚Ñ§[1/2]-trichotomous a c) Œ≥‚ÇÅ Œ≥‚ÇÇ
 where
  Œ≥‚ÇÅ : a < c ‚Üí (a < c) ‚àî (d < b)
  Œ≥‚ÇÅ = inl

  Œ≥‚ÇÇ : (a Ôºù c) ‚àî (c < a) ‚Üí (a < c) ‚àî (d < b)
  Œ≥‚ÇÇ (inl e) = inr Œ≥
   where
    I : c - b < c - d
    I = transport (Œª z ‚Üí z - b < c - d) e l‚ÇÅ

    II : (- b) < (- d)
    II = ‚Ñ§[1/2]<-addition-cancellable' (- b) c (- d) I

    III : - (- d) < - (- b)
    III = ‚Ñ§[1/2]<-swap (- b) (- d) II

    IV : - (- d) Ôºù d
    IV = ‚Ñ§[1/2]-minus-minus d ‚Åª¬π

    V : - ( - b) Ôºù b
    V = ‚Ñ§[1/2]-minus-minus b ‚Åª¬π

    Œ≥ : d < b
    Œ≥ = transport‚ÇÇ _<_ IV V III
    
  Œ≥‚ÇÇ (inr l) = inr Œ≥
   where
    I : - a < - c
    I = ‚Ñ§[1/2]<-swap c a l

    II : (- a) + (a - b) < (- c) + (c - d)
    II = ‚Ñ§[1/2]<-adding (- a) (- c) (a - b) (c - d) I l‚ÇÅ

    III : (u v : ‚Ñ§[1/2]) ‚Üí (- u) + (u - v) Ôºù - v
    III u v = (- u) + (u - v) Ôºù‚ü® ‚Ñ§[1/2]+-assoc (- u) u (- v) ‚Åª¬π             ‚ü©
              (- u) + u - v   Ôºù‚ü® ap (_- v) (‚Ñ§[1/2]+-inverse-sum-to-zero' u) ‚ü©
              0‚Ñ§[1/2] - v     Ôºù‚ü® ‚Ñ§[1/2]-zero-left-neutral (- v)             ‚ü©
              - v             ‚àé

    IV : (- a) + (a - b) Ôºù - b
    IV = III a b

    V : (- c) + (c - d) Ôºù - d
    V = III c d

    VI : - b < - d
    VI = transport‚ÇÇ _<_ IV V II

    Œ≥ : d < b
    Œ≥ = ‚Ñ§[1/2]<-swap' b d VI

‚Ñ§-distributivity-neg : (p q r : ‚Ñ§) ‚Üí p ‚Ñ§* q ‚Ñ§- p ‚Ñ§* r Ôºù p ‚Ñ§* (q ‚Ñ§- r)
‚Ñ§-distributivity-neg p q r = Œ≥
 where
  I : ‚Ñ§- p ‚Ñ§* r Ôºù p ‚Ñ§* (‚Ñ§- r)
  I = negation-dist-over-mult p r ‚Åª¬π
  
  Œ≥ : p ‚Ñ§* q ‚Ñ§- p ‚Ñ§* r Ôºù p ‚Ñ§* (q ‚Ñ§- r)
  Œ≥ = p ‚Ñ§* q ‚Ñ§- p ‚Ñ§* r      Ôºù‚ü® ap (p ‚Ñ§* q ‚Ñ§+_) I ‚ü©
      p ‚Ñ§* q ‚Ñ§+ p ‚Ñ§* (‚Ñ§- r) Ôºù‚ü® distributivity-mult-over-‚Ñ§' q (‚Ñ§- r) p ‚Åª¬π ‚ü©
      p ‚Ñ§* (q ‚Ñ§- r)         ‚àé

‚Ñ§-distributivity-neg' : (p q r : ‚Ñ§) ‚Üí p ‚Ñ§* q ‚Ñ§- r ‚Ñ§* q Ôºù (p ‚Ñ§- r) ‚Ñ§* q
‚Ñ§-distributivity-neg' p q r = Œ≥
 where
  I : ‚Ñ§- r ‚Ñ§* q Ôºù (‚Ñ§- r) ‚Ñ§* q
  I = negation-dist-over-mult' r q ‚Åª¬π
  
  Œ≥ : p ‚Ñ§* q ‚Ñ§- r ‚Ñ§* q Ôºù (p ‚Ñ§- r) ‚Ñ§* q
  Œ≥ = p ‚Ñ§* q ‚Ñ§- r ‚Ñ§* q      Ôºù‚ü® ap (p ‚Ñ§* q ‚Ñ§+_) I                        ‚ü© 
      p ‚Ñ§* q ‚Ñ§+ (‚Ñ§- r) ‚Ñ§* q Ôºù‚ü® distributivity-mult-over-‚Ñ§ p (‚Ñ§- r) q ‚Åª¬π ‚ü©
      (p ‚Ñ§- r) ‚Ñ§* q         ‚àé

2‚Ñ§[1/2] : ‚Ñ§[1/2]
2‚Ñ§[1/2] = (pos 2 , 0) , inl refl

normalise-neg-step' : (z : ‚Ñ§)  (n : ‚Ñï)
 ‚Üí normalise-neg (z , succ n) Ôºù 2‚Ñ§[1/2] * normalise-neg (z , n)
normalise-neg-step' z 0 = Œ≥
 where
  I : normalise-pos (z ‚Ñ§* pos 2 , 0) Ôºù (z ‚Ñ§* pos 2 , 0) , inl refl
  I = ‚Ñ§[1/2]-to-normalise-pos ((z ‚Ñ§* pos 2 , 0) , inl refl) ‚Åª¬π

  II : z ‚Ñ§* pos 2 ‚Ñ§* pos 2 Ôºù pos 2 ‚Ñ§* (z ‚Ñ§* pos 2)
  II = ‚Ñ§*-comm (z ‚Ñ§* pos 2) (pos 2)
  
  Œ≥ : normalise-neg (z , 1) Ôºù 2‚Ñ§[1/2] * normalise-neg (z , zero)
  Œ≥ = normalise-neg (z , 1)                           Ôºù‚ü® refl ‚ü©
      normalise-neg-lemma z 1                         Ôºù‚ü® refl ‚ü©
      normalise-neg-lemma (z ‚Ñ§* pos 2) 0              Ôºù‚ü® refl ‚ü©
      (z ‚Ñ§* pos 2 ‚Ñ§* pos 2 , 0) , inl refl            Ôºù‚ü® i    ‚ü©
      normalise-pos (z ‚Ñ§* pos 2 ‚Ñ§* pos 2 , 0)         Ôºù‚ü® ii   ‚ü©
      normalise-pos ((pos 2 ‚Ñ§* (z ‚Ñ§* pos 2)) , 0)     Ôºù‚ü® refl ‚ü©
      normalise-pos ((pos 2 , 0) *' (z ‚Ñ§* pos 2 , 0)) Ôºù‚ü® iii  ‚ü©
      2‚Ñ§[1/2] * normalise-pos (z ‚Ñ§* pos 2 , 0)        Ôºù‚ü® iv   ‚ü©
      2‚Ñ§[1/2] * ((z ‚Ñ§* pos 2 , 0) , inl refl)         Ôºù‚ü® refl ‚ü©
      2‚Ñ§[1/2] * normalise-neg-lemma z 0               Ôºù‚ü® refl ‚ü©
      2‚Ñ§[1/2] * normalise-neg (z , 0)                 ‚àé
   where
    i   = ‚Ñ§[1/2]-to-normalise-pos ((z ‚Ñ§* pos 2 ‚Ñ§* pos 2 , 0) , inl refl)
    ii  = ap (Œª - ‚Üí normalise-pos (- , 0)) II
    iii = ‚Ñ§[1/2]*-normalise-pos (pos 2 , 0) (z ‚Ñ§* pos 2 , 0)
    iv  = ap (2‚Ñ§[1/2] *_) I

normalise-neg-step' z (succ n) = Œ≥
 where
  IH : normalise-neg (z ‚Ñ§* pos 2 , succ n)
     Ôºù 2‚Ñ§[1/2] * normalise-neg (z ‚Ñ§* pos 2 , n)
  IH = normalise-neg-step' (z ‚Ñ§* pos 2) n

  I : normalise-neg (z ‚Ñ§* pos 2 , succ n)
    Ôºù 2‚Ñ§[1/2] * normalise-neg (z ‚Ñ§* pos 2 , n)
  I = normalise-neg-step' (z ‚Ñ§* pos 2) n
  
  Œ≥ : normalise-neg (z , succ (succ n)) Ôºù 2‚Ñ§[1/2] * normalise-neg (z , succ n)
  Œ≥ = normalise-neg (z , succ (succ n))            Ôºù‚ü® refl ‚ü©
      normalise-neg-lemma z (succ (succ n))        Ôºù‚ü® refl ‚ü©
      normalise-neg-lemma (z ‚Ñ§* pos 2) (succ n)    Ôºù‚ü® refl ‚ü©
      normalise-neg-lemma (z ‚Ñ§* pos 2 ‚Ñ§* pos 2) n  Ôºù‚ü® I    ‚ü©
      2‚Ñ§[1/2] * normalise-neg-lemma (z ‚Ñ§* pos 2) n Ôºù‚ü® refl ‚ü©
      2‚Ñ§[1/2] * normalise-neg-lemma z (succ n)     Ôºù‚ü® refl ‚ü©      
      2‚Ñ§[1/2] * normalise-neg (z , succ n)         ‚àé

normalise-neg-step : ((z , n) : ‚Ñ§ √ó ‚Ñï)
 ‚Üí normalise-neg (z , succ n) Ôºù 2‚Ñ§[1/2] * normalise-neg (z , n)
normalise-neg-step (z , n) = normalise-neg-step' z n

normalise-pos-step' : (z : ‚Ñ§) (n : ‚Ñï)
 ‚Üí normalise-pos (pos 2 ‚Ñ§* z , n) Ôºù 2‚Ñ§[1/2] * normalise-pos (z , n)
normalise-pos-step' z n = Œ≥
 where
  Œ≥ : normalise-pos (pos 2 ‚Ñ§* z , n) Ôºù 2‚Ñ§[1/2] * normalise-pos (z , n)
  Œ≥ = normalise-pos (pos 2 ‚Ñ§* z , n)         Ôºù‚ü® i    ‚ü©
      normalise-pos (pos 2 ‚Ñ§* z , 0 ‚Ñï+ n)    Ôºù‚ü® refl ‚ü©
      normalise-pos ((pos 2 , 0) *' (z , n)) Ôºù‚ü® ii   ‚ü©
      2‚Ñ§[1/2] * normalise-pos (z , n)        ‚àé
   where
    i  = ap (Œª - ‚Üí normalise-pos (pos 2 ‚Ñ§* z , -)) (zero-left-neutral n ‚Åª¬π)
    ii = ‚Ñ§[1/2]*-normalise-pos (pos 2 , 0) (z , n)

normalise-pos-step : ((z , n) : ‚Ñ§ √ó ‚Ñï)
 ‚Üí normalise-pos (pos 2 ‚Ñ§* z , n) Ôºù 2‚Ñ§[1/2] * normalise-pos (z , n)
normalise-pos-step (z , n) = normalise-pos-step' z n

normalise-neg-to-pos' : (z : ‚Ñ§) (n : ‚Ñï)
                     ‚Üí normalise-neg (z , n)
                     Ôºù normalise-pos (pos (2^ (succ n)) ‚Ñ§* z , 0)
normalise-neg-to-pos' z 0      = Œ≥
 where
  Œ≥ : normalise-neg (z , 0) Ôºù normalise-pos (pos (2^ 1) ‚Ñ§* z , 0)
  Œ≥ = normalise-neg (z , 0)               Ôºù‚ü® refl ‚ü©
      (z ‚Ñ§+ z , 0) , inl refl             Ôºù‚ü® refl ‚ü©
      normalise-pos (z ‚Ñ§+ z , 0)          Ôºù‚ü® refl ‚ü©
      normalise-pos (z ‚Ñ§* pos 2 , 0)      Ôºù‚ü® i    ‚ü©
      normalise-pos (pos 2 ‚Ñ§* z , 0)      Ôºù‚ü® refl ‚ü©
      normalise-pos (pos (2^ 1) ‚Ñ§* z , 0) ‚àé
   where
    i = ap (Œª - ‚Üí normalise-pos (- , 0)) (‚Ñ§*-comm z (pos 2))
normalise-neg-to-pos' z (succ n) = Œ≥
 where
  IH : normalise-neg (z , n) Ôºù normalise-pos (pos (2^ (succ n)) ‚Ñ§* z , 0)
  IH = normalise-neg-to-pos' z n

  n' = pos (2^ (succ n))

  Œ≥ : normalise-neg (z , succ n)
    Ôºù normalise-pos (pos (2^ (succ (succ n))) ‚Ñ§* z , 0)
  Œ≥ = normalise-neg (z , succ n)                        Ôºù‚ü® i    ‚ü©
      2‚Ñ§[1/2] * normalise-neg (z , n)                   Ôºù‚ü® ii   ‚ü©
      2‚Ñ§[1/2] * normalise-pos (n' ‚Ñ§* z , 0)             Ôºù‚ü® iii  ‚ü©
      normalise-pos (pos 2 ‚Ñ§* (n' ‚Ñ§* z) , 0)            Ôºù‚ü® iv   ‚ü©
      normalise-pos (pos 2 ‚Ñ§* n' ‚Ñ§* z , 0)              Ôºù‚ü® v    ‚ü©
      normalise-pos (pos (2 ‚Ñï* 2^ (succ n)) ‚Ñ§* z , 0)   Ôºù‚ü® refl ‚ü©
      normalise-pos (pos (2^ (succ (succ n))) ‚Ñ§* z , 0) ‚àé
   where
    v‚Çê‚Çö : pos 2 ‚Ñ§* pos (2^ (succ n)) Ôºù pos (2 ‚Ñï* 2^ (succ n))
    v‚Çê‚Çö = pos-multiplication-equiv-to-‚Ñï 2 (2^ (succ n))
    
    i   = normalise-neg-step (z , n)
    ii  = ap (2‚Ñ§[1/2] *_) IH
    iii = normalise-pos-step (n' ‚Ñ§* z , 0) ‚Åª¬π
    iv  = ap (Œª - ‚Üí normalise-pos (- , 0)) (‚Ñ§*-assoc (pos 2) n' z ‚Åª¬π)
    v   = ap (Œª - ‚Üí normalise-pos (- ‚Ñ§* z , 0)) v‚Çê‚Çö

normalise-neg-to-pos : ((z , n) : ‚Ñ§ √ó ‚Ñï)
                     ‚Üí normalise-neg (z , n)
                     Ôºù normalise-pos (pos (2^ (succ n)) ‚Ñ§* z , 0)
normalise-neg-to-pos (z , n) = normalise-neg-to-pos' z n

normalise-pos-negation : (p q : ‚Ñ§) ‚Üí (n : ‚Ñï)
                       ‚Üí normalise-pos (p , n) - normalise-pos (q , n)
                       Ôºù normalise-pos (p ‚Ñ§- q , n)
normalise-pos-negation p q n = Œ≥
 where
  n' = pos (2^ n)

  I : (‚Ñ§- q) ‚Ñ§* n' Ôºù ‚Ñ§- q ‚Ñ§* n'
  I = negation-dist-over-mult' q n'

  II : p ‚Ñ§* n' ‚Ñ§- q ‚Ñ§* n' Ôºù (p ‚Ñ§- q) ‚Ñ§* n'
  II = ‚Ñ§-distributivity-neg' p n' q

  III : n' ‚Ñ§* n' Ôºù pos (2^ (n ‚Ñï+ n))
  III = n' ‚Ñ§* n'            Ôºù‚ü® pos-multiplication-equiv-to-‚Ñï (2^ n) (2^ n) ‚ü©
        pos (2^ n ‚Ñï* 2^ n)  Ôºù‚ü® ap pos (prod-of-powers 2 n n)               ‚ü©
        pos (2^ (n ‚Ñï+ n))   ‚àé
  
  IV : ((p , n) +' (‚Ñ§- q , n)) ‚âà' (p ‚Ñ§- q , n)
  IV = (p ‚Ñ§* n' ‚Ñ§+ (‚Ñ§- q) ‚Ñ§* n') ‚Ñ§* n' Ôºù‚ü® ap (Œª z ‚Üí (p ‚Ñ§* n' ‚Ñ§+ z) ‚Ñ§* n') I ‚ü©
       (p ‚Ñ§* n' ‚Ñ§- q ‚Ñ§* n') ‚Ñ§* n'      Ôºù‚ü® ap (_‚Ñ§* n') II                    ‚ü©
       (p ‚Ñ§- q) ‚Ñ§* n' ‚Ñ§* n'            Ôºù‚ü® ‚Ñ§*-assoc (p ‚Ñ§- q) n' n'           ‚ü©
       (p ‚Ñ§- q) ‚Ñ§* (n' ‚Ñ§* n')          Ôºù‚ü® ap ((p ‚Ñ§- q) ‚Ñ§*_) III             ‚ü©
       (p ‚Ñ§- q) ‚Ñ§* pos (2^ (n ‚Ñï+ n))   ‚àé

  Œ≥ : normalise-pos (p , n) - normalise-pos (q , n) Ôºù normalise-pos (p ‚Ñ§- q , n)
  Œ≥ = normalise-pos (p , n) - normalise-pos (q , n)     Ôºù‚ü® refl ‚ü©
      normalise-pos (p , n) + (- normalise-pos (q , n)) Ôºù‚ü® i    ‚ü©
      normalise-pos (p , n) + normalise-pos (‚Ñ§- q , n)  Ôºù‚ü® ii   ‚ü©
      normalise-pos ((p , n) +' (‚Ñ§- q , n))             Ôºù‚ü® iii  ‚ü©
      normalise-pos (p ‚Ñ§- q , n)                        ‚àé
   where
    i   = ap (normalise-pos (p , n) +_) (minus-normalise-pos q n)
    ii  = ‚Ñ§[1/2]+-normalise-pos (p , n) (‚Ñ§- q , n) ‚Åª¬π
    iii = ‚âà'-to-Ôºù ((p , n) +' (‚Ñ§- q , n)) (p ‚Ñ§- q , n) IV

normalise-negation :
 (p q n : ‚Ñ§) ‚Üí normalise (p , n) - normalise (q , n) Ôºù normalise (p ‚Ñ§- q , n)
normalise-negation p q (pos n) = normalise-pos-negation p q n
normalise-negation p q (negsucc n) = Œ≥
 where
  n' = pos (2^ (succ n))
  
  Œ≥ : normalise (p , negsucc n) - normalise (q , negsucc n)
    Ôºù normalise (p ‚Ñ§- q , negsucc n)
  Œ≥ = normalise (p , negsucc n) - normalise (q , negsucc n)     Ôºù‚ü® i   ‚ü©
      normalise-pos (n' ‚Ñ§* p , 0) - normalise (q , negsucc n)   Ôºù‚ü® ii  ‚ü©
      normalise-pos (n' ‚Ñ§* p , 0) - normalise-pos (n' ‚Ñ§* q , 0) Ôºù‚ü® iii ‚ü©
      normalise-pos (n' ‚Ñ§* p ‚Ñ§- n' ‚Ñ§* q , 0)                    Ôºù‚ü® iv  ‚ü©
      normalise-pos (n' ‚Ñ§* (p ‚Ñ§- q) , 0)                        Ôºù‚ü® v   ‚ü©
      normalise (p ‚Ñ§- q , negsucc n)                            ‚àé
   where
    ii‚Çê‚Çö : normalise-neg (q , n) Ôºù normalise-pos (pos (2^ (succ n)) ‚Ñ§* q , 0)
    ii‚Çê‚Çö = normalise-neg-to-pos (q , n)
    
    i   = ap (_- normalise (q , negsucc n)) (normalise-neg-to-pos (p , n))
    ii  = ap (Œª z ‚Üí normalise-pos (n' ‚Ñ§* p , 0) - z) ii‚Çê‚Çö
    iii = normalise-pos-negation (n' ‚Ñ§* p) (n' ‚Ñ§* q) 0
    iv  = ap (Œª z ‚Üí normalise-pos (z , 0)) (‚Ñ§-distributivity-neg n' p q)
    v   = normalise-neg-to-pos (p ‚Ñ§- q , n) ‚Åª¬π

normalise-negation' : (z n : ‚Ñ§) ‚Üí - normalise (z , n) Ôºù normalise (‚Ñ§- z , n)
normalise-negation' z (pos n)     = minus-normalise-pos z n
normalise-negation' z (negsucc n) = Œ≥
 where
  I : ‚Ñ§- pos (2^ (succ n)) ‚Ñ§* z Ôºù pos (2^ (succ n)) ‚Ñ§* (‚Ñ§- z)
  I = negation-dist-over-mult (pos (2^ (succ n))) z ‚Åª¬π
  
  Œ≥ : - normalise (z , negsucc n) Ôºù normalise (‚Ñ§- z , negsucc n)
  Œ≥ = - normalise (z , negsucc n)                     Ôºù‚ü® refl ‚ü©
      - normalise-neg (z , n)                         Ôºù‚ü® i    ‚ü©
      - normalise-pos (pos (2^ (succ n)) ‚Ñ§* z , 0)    Ôºù‚ü® ii   ‚ü©
      normalise-pos (‚Ñ§- pos (2^ (succ n)) ‚Ñ§* z , 0)   Ôºù‚ü® iii  ‚ü©
      normalise-pos (pos (2^ (succ n)) ‚Ñ§* (‚Ñ§- z) , 0) Ôºù‚ü® iv   ‚ü©      
      normalise-neg (‚Ñ§- z , n) Ôºù‚ü® refl ‚ü©
      normalise (‚Ñ§- z , negsucc n) ‚àé
   where
    i   = ap -_ (normalise-neg-to-pos (z , n))
    ii  = minus-normalise-pos (pos (2^ (succ n)) ‚Ñ§* z) 0
    iii = ap (Œª - ‚Üí normalise-pos (- , 0)) I
    iv  = normalise-neg-to-pos (‚Ñ§- z , n) ‚Åª¬π

normalise-pos-succ : (z : ‚Ñ§) (n : ‚Ñï) ‚Üí normalise-pos (z , n) Ôºù normalise-pos (z ‚Ñ§+ z , succ n)
normalise-pos-succ z n = ‚âà'-to-Ôºù (z , n) (z ‚Ñ§+ z , succ n) Œ≥
 where
  I : pos (2 ‚Ñï* 2^ n) Ôºù pos 2 ‚Ñ§* pos (2^ n)
  I = pos-multiplication-equiv-to-‚Ñï 2 (2^ n) ‚Åª¬π
  
  Œ≥ : (z , n) ‚âà' (z ‚Ñ§+ z , succ n)
  Œ≥ = z ‚Ñ§* pos (2^ (succ n))     Ôºù‚ü® refl                               ‚ü©
      z ‚Ñ§* pos (2 ‚Ñï* 2^ n)       Ôºù‚ü® ap (z ‚Ñ§*_) I                       ‚ü©
      z ‚Ñ§* (pos 2 ‚Ñ§* pos (2^ n)) Ôºù‚ü® ‚Ñ§*-assoc z (pos 2) (pos (2^ n)) ‚Åª¬π ‚ü©
      z ‚Ñ§* pos 2 ‚Ñ§* pos (2^ n)   Ôºù‚ü® refl                               ‚ü©
      (z ‚Ñ§+ z) ‚Ñ§* pos (2^ n)     ‚àé

normalise-succ' : (z n : ‚Ñ§) ‚Üí normalise (z , n) Ôºù normalise (z ‚Ñ§+ z , succ‚Ñ§ n)
normalise-succ' z (pos n)     = normalise-pos-succ z n
normalise-succ' z (negsucc 0) = Œ≥
 where
  I : pos 2 ‚Ñ§* z Ôºù z ‚Ñ§* pos 2
  I = ‚Ñ§*-comm (pos 2) z
  
  Œ≥ : normalise (z , negsucc 0) Ôºù normalise (z ‚Ñ§+ z , pos 0)
  Œ≥ = normalise (z , negsucc 0)      Ôºù‚ü® refl                               ‚ü©
      normalise-neg (z , 0)          Ôºù‚ü® normalise-neg-to-pos (z , 0)       ‚ü©
      normalise-pos (pos 2 ‚Ñ§* z , 0) Ôºù‚ü® ap (Œª - ‚Üí normalise-pos (- , 0)) I ‚ü©
      normalise-pos (z ‚Ñ§+ z , 0)     Ôºù‚ü® refl                               ‚ü©
      normalise (z ‚Ñ§+ z , pos 0)     ‚àé
normalise-succ' z (negsucc (succ x)) = Œ≥
 where
  I : pos (2^ (succ (succ x))) ‚Ñ§* z Ôºù pos (2^ (succ x)) ‚Ñ§* (z ‚Ñ§+ z)
  I = pos (2^ (succ (succ x))) ‚Ñ§* z     Ôºù‚ü® refl ‚ü©
      pos (2 ‚Ñï* 2^ (succ x)) ‚Ñ§* z       Ôºù‚ü® i    ‚ü©
      pos 2 ‚Ñ§* pos (2^ (succ x)) ‚Ñ§* z   Ôºù‚ü® ii   ‚ü©
      pos (2^ (succ x)) ‚Ñ§* pos 2 ‚Ñ§* z   Ôºù‚ü® iii  ‚ü©
      pos (2^ (succ x)) ‚Ñ§* (pos 2 ‚Ñ§* z) Ôºù‚ü® iv   ‚ü©
      pos (2^ (succ x)) ‚Ñ§* (z ‚Ñ§+ z)     ‚àé
   where
    i   = ap (_‚Ñ§* z) (pos-multiplication-equiv-to-‚Ñï 2 (2^ (succ x)) ‚Åª¬π)
    ii  = ap (_‚Ñ§* z) (‚Ñ§*-comm (pos 2) (pos (2^ (succ x))))
    iii = ‚Ñ§*-assoc (pos (2^ (succ x))) (pos 2) z
    iv  = ap (pos (2^ (succ x)) ‚Ñ§*_) (‚Ñ§*-comm (pos 2) z)
  
  Œ≥ : normalise (z , negsucc (succ x))
    Ôºù normalise (z ‚Ñ§+ z , succ‚Ñ§ (negsucc (succ x)))
  Œ≥ = normalise (z , negsucc (succ x))                  Ôºù‚ü® refl ‚ü©
      normalise-neg (z , succ x)                        Ôºù‚ü® i    ‚ü©
      normalise-pos (pos (2^ (succ (succ x))) ‚Ñ§* z , 0) Ôºù‚ü® ii   ‚ü©
      normalise-pos (pos (2^ (succ x)) ‚Ñ§* (z ‚Ñ§+ z) , 0) Ôºù‚ü® iii  ‚ü©
      normalise-neg (z ‚Ñ§+ z , x)                        Ôºù‚ü® refl ‚ü©      
      normalise (z ‚Ñ§+ z , succ‚Ñ§ (negsucc (succ x)))     ‚àé
   where
    i   = normalise-neg-to-pos (z , succ x)
    ii  = ap (Œª - ‚Üí normalise-pos (- , 0)) I
    iii = normalise-neg-to-pos (z ‚Ñ§+ z , x) ‚Åª¬π

normalise-pred' : (z n : ‚Ñ§)
                ‚Üí normalise (z , pred‚Ñ§ n) Ôºù normalise (pos 2 ‚Ñ§* z , n)
normalise-pred' z n = Œ≥
 where
  I : normalise (z , pred‚Ñ§ n) Ôºù normalise (z ‚Ñ§+ z , succ‚Ñ§ (pred‚Ñ§ n))
  I = normalise-succ' z (pred‚Ñ§ n)
  
  Œ≥ : normalise (z , pred‚Ñ§ n) Ôºù normalise (pos 2 ‚Ñ§* z , n)
  Œ≥ = normalise (z , pred‚Ñ§ n)              Ôºù‚ü® i   ‚ü©
      normalise (z ‚Ñ§+ z , succ‚Ñ§ (pred‚Ñ§ n)) Ôºù‚ü® ii  ‚ü©
      normalise (z ‚Ñ§+ z , n)               Ôºù‚ü® iii ‚ü©
      normalise (pos 2 ‚Ñ§* z , n)           ‚àé
   where
    i   = normalise-succ' z (pred‚Ñ§ n)
    ii  = ap (Œª - ‚Üí normalise (z ‚Ñ§+ z , -)) (succpred‚Ñ§ n)
    iii = ap (Œª - ‚Üí normalise (- , n)) (‚Ñ§*-comm z (pos 2))

normalise-‚â§-prop2 : (p q n : ‚Ñ§) ‚Üí p ‚â§ q ‚Üí normalise (p , n) ‚â§ normalise (q , n)
normalise-‚â§-prop2 p q (pos n) l = normalise-pos-‚â§ (p , n) (q , n) Œ≥
 where
  I : is-pos-succ (pos (2^ n))
  I = exponents-of-two-positive n
 
  Œ≥ : p ‚Ñ§* pos (2^ n) ‚â§ q ‚Ñ§* pos (2^ n)
  Œ≥ = positive-multiplication-preserves-order' p q (pos (2^ n)) I l
normalise-‚â§-prop2 p q (negsucc n) l = Œ≥ 
 where
  I : normalise-pos (pos (2^ (succ n)) ‚Ñ§* p , 0) Ôºù normalise-neg (p , n)
  I = normalise-neg-to-pos (p , n) ‚Åª¬π
  
  II : normalise-pos (pos (2^ (succ n)) ‚Ñ§* q , 0) Ôºù normalise-neg (q , n)
  II = normalise-neg-to-pos (q , n) ‚Åª¬π

  III : is-pos-succ (pos (2^ (succ n)))
  III = exponents-of-two-positive (succ n)

  IV : p ‚Ñ§* pos (2^ (succ n)) ‚â§ q ‚Ñ§* pos (2^ (succ n))
  IV = positive-multiplication-preserves-order' p q (pos (2^ (succ n))) III l

  V : pos (2^ (succ n)) ‚Ñ§* p ‚â§ pos (2^ (succ n)) ‚Ñ§* q
  V = transport‚ÇÇ _‚â§_ i ii IV
   where
    i : p ‚Ñ§* pos (2^ (succ n)) Ôºù pos (2^ (succ n)) ‚Ñ§* p
    i = ‚Ñ§*-comm p (pos (2^ (succ n)))

    ii : q ‚Ñ§* pos (2^ (succ n)) Ôºù pos (2^ (succ n)) ‚Ñ§* q
    ii = ‚Ñ§*-comm q (pos (2^ (succ n)))
  
  Œ≥' : normalise-pos (pos (2^ (succ n)) ‚Ñ§* p , 0)
      ‚â§ normalise-pos (pos (2^ (succ n)) ‚Ñ§* q , 0)
  Œ≥' = normalise-pos-‚â§
        (pos (2^ (succ n)) ‚Ñ§* p , 0)
        (pos (2^ (succ n)) ‚Ñ§* q , 0)
        V

  Œ≥ : normalise-neg (p , n) ‚â§ normalise-neg (q , n)
  Œ≥ = transport‚ÇÇ _‚â§_ I II Œ≥'

normalise-‚â§-prop : (n : ‚Ñï) ‚Üí ((k , p) : ‚Ñ§ √ó ‚Ñ§)
                 ‚Üí normalise (k , p) ‚â§ normalise (k ‚Ñ§+ pos n , p)
normalise-‚â§-prop n (k , p) = normalise-‚â§-prop2 k (k ‚Ñ§+ pos n) p (n , refl)



postulate
 from-normalise-‚â§-same-denom :
  (a b c : ‚Ñ§) ‚Üí normalise (a , c) ‚â§ normalise (b , c) ‚Üí a ‚â§ b
 ‚Ñ§[1/2]-find-lower :
  (Œµ : ‚Ñ§[1/2]) ‚Üí ‚Ñ§[1/2]-is-positive Œµ ‚Üí Œ£ n Íûâ ‚Ñ§ , normalise (pos 2 , n) < Œµ
 ‚Ñ§[1/2]<-1/2' : (p : ‚Ñ§[1/2]) ‚Üí 0‚Ñ§[1/2] < p ‚Üí 1/2‚Ñ§[1/2] * p < p

```
