```agda
{-# OPTIONS --without-K --exact-split #-}

open import UF.FunExt
open import MLTT.Spartan

module Todd.TernaryBoehmRealsPrelude where

open import MLTT.Two-Properties hiding (zero-is-not-one)
open import Naturals.Order
open import Naturals.Addition renaming (_+_ to _+â„•_)
open import Naturals.Multiplication renaming (_*_ to _â„•*_)
open import Integers.Type
open import Integers.Order
open import Integers.Addition renaming (_+_ to _+â„¤_ ; _-_ to _â„¤-_)
open import Integers.Multiplication renaming (_*_ to _â„¤*_)
open import Integers.Negation renaming (-_  to  âˆ’â„¤_)
open import UF.Subsingletons
open import Naturals.Order
open import NotionsOfDecidability.DecidableAndDetachable
open import Notation.Order

succ-lc : (x y : â„•) â†’ succ x ï¼ succ y â†’ x ï¼ y
succ-lc x x refl = refl

â„•-is-discrete : (x y : â„•) â†’ decidable (x ï¼ y)
â„•-is-discrete zero zero = inl refl
â„•-is-discrete zero (succ y) = inr (Î» ())
â„•-is-discrete (succ x) zero = inr (Î» ())
â„•-is-discrete (succ x) (succ y)
 = Cases (â„•-is-discrete x y)
     (inl âˆ˜ ap succ)
     (inr âˆ˜ Î» f g â†’ f (succ-lc x y g))

_â‰¤â„¤_â‰¤â„¤_ : â„¤ â†’ â„¤ â†’ â„¤ â†’ ğ“¤â‚€ Ì‡ 
x â‰¤â„¤ y â‰¤â„¤ z = (x â‰¤â„¤ y) Ã— (y â‰¤â„¤ z)

â‰¤â„¤Â²-is-prop : {l u : â„¤} (x : â„¤) â†’ is-prop (l â‰¤â„¤ x â‰¤â„¤ u)
â‰¤â„¤Â²-is-prop {l} {u} x = Ã—-is-prop (â„¤â‰¤-is-prop l x) (â„¤â‰¤-is-prop x u)

data ğŸ› : ğ“¤â‚€ Ì‡ where
  âˆ’1 O +1 : ğŸ›

_/2 : â„• â†’ â„•
0 /2 = 0
1 /2 = 0
succ (succ n) /2 = succ (n /2)

_/2' : â„¤ â†’ â„¤
pos x     /2' = pos (x /2)
negsucc x /2' = âˆ’â„¤ (pos (succ x /2))

sign : â„¤ â†’ (â„• â†’ â„¤)
sign (pos     _) = pos
sign (negsucc _) = negsucc

num : â„¤ â†’ â„•
num  (pos     n) = n
num  (negsucc n) = n

odd even : â„¤ â†’ ğ“¤â‚€ Ì‡
odd (pos                   0) = ğŸ˜
odd (pos                   1) = ğŸ™
odd (pos (succ (succ x)))     = odd (pos x)
odd (negsucc               0) = ğŸ™
odd (negsucc               1) = ğŸ˜
odd (negsucc (succ (succ x))) = odd (negsucc x)
even x = Â¬ odd x

even-or-odd? : (x : â„¤) â†’ even x + odd x
even-or-odd? (pos                   0) = inl (Î» x â†’ x)
even-or-odd? (pos                   1) = inr â‹†
even-or-odd? (pos (succ (succ x)))     = even-or-odd? (pos x)
even-or-odd? (negsucc               0) = inr â‹†
even-or-odd? (negsucc               1) = inl (Î» x â†’ x)
even-or-odd? (negsucc (succ (succ x))) = even-or-odd? (negsucc x)

odd-is-prop : (x : â„¤) â†’ is-prop (odd x)
odd-is-prop (pos                   0) = ğŸ˜-is-prop
odd-is-prop (pos                   1) = ğŸ™-is-prop
odd-is-prop (pos (succ (succ x)))     = odd-is-prop (pos x)
odd-is-prop (negsucc               0) = ğŸ™-is-prop
odd-is-prop (negsucc               1) = ğŸ˜-is-prop
odd-is-prop (negsucc (succ (succ x))) = odd-is-prop (negsucc x)

succ-odd-is-even : (x : â„¤) â†’ odd x â†’ even (succâ„¤ x)
succ-odd-is-even (pos                          1) o = id
succ-odd-is-even (pos            (succ (succ x))) o = succ-odd-is-even (pos x) o
succ-odd-is-even (negsucc                      0) o = id
succ-odd-is-even (negsucc (succ (succ (succ x)))) o = succ-odd-is-even (negsucc (succ x)) o

succ-even-is-odd : (x : â„¤) â†’ even x â†’ odd (succâ„¤ x)
succ-even-is-odd (pos                          0) e = â‹†
succ-even-is-odd (pos                          1) e = e â‹†
succ-even-is-odd (pos            (succ (succ x))) e = succ-even-is-odd (pos x) e
succ-even-is-odd (negsucc                      0) e = e â‹†
succ-even-is-odd (negsucc                      1) e = â‹†
succ-even-is-odd (negsucc                      2) e = e â‹†
succ-even-is-odd (negsucc (succ (succ (succ x)))) e = succ-even-is-odd (negsucc (succ x)) e

odd-succ-succ : (x : â„¤) â†’ odd x â†’ odd (succâ„¤ (succâ„¤ x))
odd-succ-succ (pos x) = id
odd-succ-succ (negsucc zero) = id
odd-succ-succ (negsucc (succ (succ x))) = id

even-succ-succ : (x : â„¤) â†’ even x â†’ even (succâ„¤ (succâ„¤ x))
even-succ-succ (pos x) = id
even-succ-succ (negsucc zero) = id
even-succ-succ (negsucc (succ (succ x))) = id

-- even-is-prop : (x : â„¤) â†’ is-prop (even x)
-- even-is-prop x p q = dfunext (fe _ _) (Î» i â†’ ğŸ˜-elim (p i))

-- even-or-odd-is-prop : (x : â„¤) â†’ is-prop (even x + odd x)
-- even-or-odd-is-prop x = +-is-prop (even-is-prop x) (odd-is-prop x) id

_âˆ’â„¤_ : â„¤ â†’ â„¤ â†’ â„¤
x âˆ’â„¤ y = x +â„¤ (âˆ’â„¤ y)

â„¤[_,_] : â„¤ â†’ â„¤ â†’ ğ“¤â‚€ Ì‡
â„¤[ l , u ] = Î£ z ê‰ â„¤ , (l â‰¤â„¤ z â‰¤â„¤ u)

â„¤[_,_]-succ : (l u : â„¤) â†’ â„¤[ l , u ] â†’ â„¤[ l , succâ„¤ u ]
â„¤[ l , u ]-succ (z , lâ‰¤z , zâ‰¤u) = z , lâ‰¤z , â„¤â‰¤-trans z u (succâ„¤ u) zâ‰¤u (1 , refl) 

â‰¤â„¤-antisym : âˆ€ x y â†’ x â‰¤â„¤ y â‰¤â„¤ x â†’ x ï¼ y
â‰¤â„¤-antisym x y (xâ‰¤y , yâ‰¤x) with â„¤â‰¤-split x y xâ‰¤y | â„¤â‰¤-split y x yâ‰¤x
... | inl (n , Î³) | inl (m , Î´)
 = ğŸ˜-elim (â„¤-equal-not-less-than x (â„¤<-trans x y x (n , Î³) (m , Î´)))
... | inl  _  | inr yï¼x = yï¼x â»Â¹
... | inr xï¼y | _       = xï¼y

â‰¤â„¤-back : âˆ€ x y â†’ x <â„¤ y â†’ x â‰¤â„¤ predâ„¤ y
â‰¤â„¤-back x .(succâ„¤ x +â„¤ pos n) (n , refl)
 = â„¤â‰¤-trans x (x +pos n) (predâ„¤ (succâ„¤ x +pos n))
     (n , refl)
     (transport ((x +pos n) â‰¤â„¤_)
       (predsuccâ„¤ (x +pos n) â»Â¹
       âˆ™ ap predâ„¤ (â„¤-left-succ x (pos n) â»Â¹))
       (â„¤â‰¤-refl (x +pos n)))

â„¤-dich-succ : (x y : â„¤) 
            â†’ ((      x <â„¤ y) + (y â‰¤â„¤       x))
            â†’ ((succâ„¤ x <â„¤ y) + (y â‰¤â„¤ succâ„¤ x))
â„¤-dich-succ x y (inl (0 , refl)) = inr (â„¤â‰¤-refl _)
â„¤-dich-succ x y (inl (succ m , refl)) = inl (m , â„¤-left-succ-pos (succâ„¤ x) m)
â„¤-dich-succ x y (inr (m , refl)) = inr (succ m , refl)

â„¤-trich-succ : (x y : â„¤) 
             â†’ ((      x <â„¤ y) + (      x ï¼ y) + (y <â„¤       x))
             â†’ ((succâ„¤ x <â„¤ y) + (succâ„¤ x ï¼ y) + (y <â„¤ succâ„¤ x))
â„¤-trich-succ x y (inl (0           , sn+jï¼i))
 = (inr âˆ˜ inl) sn+jï¼i
â„¤-trich-succ x y (inl (succ j      , sn+jï¼i))
 = inl (j , (â„¤-left-succ-pos (succâ„¤ x) j âˆ™ sn+jï¼i))
â„¤-trich-succ x y (inr (inl              nï¼i))
 = (inr âˆ˜ inr) (0 , ap succâ„¤ (nï¼i â»Â¹))
â„¤-trich-succ x y (inr (inr (j      , sn+jï¼i)))
 = (inr âˆ˜ inr) (succ j , ap succâ„¤ sn+jï¼i)

â„¤-vert-trich-locate : â„¤ â†’ â„¤ â†’ â„¤ â†’ ğ“¤â‚€ Ì‡
â„¤-vert-trich-locate z a b = (z <â„¤ a) + (a â‰¤â„¤ z â‰¤â„¤ b) + (b <â„¤ z)

â„¤-vert-trich-succ : (z a b : â„¤) â†’ a <â„¤ b
                  â†’ â„¤-vert-trich-locate        z  a b
                  â†’ â„¤-vert-trich-locate (succâ„¤ z) a b
â„¤-vert-trich-succ z a b (k , Î·) (inl (succ n , Îµ))
 = inl         (n , (â„¤-left-succ-pos (succâ„¤ z) n âˆ™ Îµ))
â„¤-vert-trich-succ z a b (k , Î·) (inl (0      , refl))
 = (inr âˆ˜ inl) ((0 , refl) , (succ k , (â„¤-left-succ-pos (succâ„¤ z) k â»Â¹ âˆ™ Î·)))
â„¤-vert-trich-succ z a b (k , Î·) (inr (inl ((nâ‚ , Îµâ‚) , succ nâ‚‚ , Îµâ‚‚)))
 = (inr âˆ˜ inl) ((succ nâ‚ , (ap succâ„¤ Îµâ‚)) , (nâ‚‚ , (â„¤-left-succ-pos z nâ‚‚ âˆ™ Îµâ‚‚)))
â„¤-vert-trich-succ z a b (k , Î·) (inr (inl ((nâ‚ , Îµâ‚) , zero , Îµâ‚‚)))
 = (inr âˆ˜ inr) (0 , ap succâ„¤ (Îµâ‚‚ â»Â¹))
â„¤-vert-trich-succ z a b (k , Î·) (inr (inr (n , refl)))
 = (inr âˆ˜ inr) (succ n , refl)

â„¤-vert-trich-all : (z a b : â„¤) â†’ â„¤-vert-trich-locate z a b
â„¤-vert-trich-all z a b = Cases (â„¤-trichotomous z a) inl
                 Î» aâ‰¤z â†’ Cases (â„¤-trichotomous b z) (inr âˆ˜ inr)
                 Î» zâ‰¤b â†’ (inr âˆ˜ inl) (â„¤â‰¤-attach _ _ aâ‰¤z , â„¤â‰¤-attach _ _ zâ‰¤b)

â„¤-vert-trich-is-prop : (z a b : â„¤) â†’ a <â„¤ b â†’ is-prop (â„¤-vert-trich-locate z a b)
â„¤-vert-trich-is-prop z a b a<b
 = +-is-prop (â„¤<-is-prop z a) (+-is-prop (â‰¤â„¤Â²-is-prop z) (â„¤<-is-prop b z)
     (Î» (_ , zâ‰¤b) â†’ â„¤-bigger-or-equal-not-less z b zâ‰¤b))
    (Î» z<a â†’ cases
     (Î» (aâ‰¤z , _) â†’ â„¤-less-not-bigger-or-equal z a z<a aâ‰¤z)
     (â„¤-bigger-or-equal-not-less z b (<-is-â‰¤ z b (â„¤<-trans z a b z<a a<b))))

ne : (a b c : â„¤)
   â†’ ((n , _) : a â‰¤ c) â†’ ((nâ‚ , _) : a â‰¤ b) â†’ ((nâ‚‚ , _) : b â‰¤ c)
   â†’ nâ‚ +â„• nâ‚‚ ï¼ n
ne a b c aâ‰¤c aâ‰¤b bâ‰¤c = â„¤â‰¤-same-witness a c (â„¤â‰¤-trans a b c aâ‰¤b bâ‰¤c) aâ‰¤c

ye : (a b c : â„¤) â†’ ((n , _) : a â‰¤ c) â†’ a â‰¤ b â†’ ((nâ‚‚ , _) : b â‰¤ c) â†’ nâ‚‚ <â„• succ n
ye a b c (n , q) (nâ‚ , r) (nâ‚‚ , s)
 = transport (nâ‚‚ â‰¤â„•_) (ne a b c (n , q) (nâ‚ , r) (nâ‚‚ , s)) (â‰¤-+' nâ‚ nâ‚‚)

rec-f-ï¼ : {X : ğ“¤ Ì‡ } â†’ (f : X â†’ X) (x : X) (n : â„•)
        â†’ rec (f x) f n ï¼ rec x f (succ n) 
rec-f-ï¼ f x zero = refl
rec-f-ï¼ f x (succ n) = ap f (rec-f-ï¼ f x n)

â„¤â‰¤Â²-refl : (k : â„¤) â†’ k â‰¤â„¤ k â‰¤â„¤ k
â„¤â‰¤Â²-refl k = â„¤â‰¤-refl k , â„¤â‰¤-refl k

_â„•^_ : â„• â†’ â„• â†’ â„•
a â„•^ b = ((a â„•*_) ^ b) 1

infixl 33 _â„•^_ 

2^ : â„• â†’ â„•
2^ = 2 â„•^_

negation-preserves-parity : (x : â„¤) â†’ even x â†’ even (âˆ’â„¤ x)
negation-preserves-parity (pos 0) = id
negation-preserves-parity (pos (succ 0)) e = ğŸ˜-elim (e â‹†)
negation-preserves-parity (pos (succ (succ 0))) e = id
negation-preserves-parity (pos (succ (succ (succ x)))) e = negation-preserves-parity (pos (succ x)) e
negation-preserves-parity (negsucc 0) e = ğŸ˜-elim (e â‹†)
negation-preserves-parity (negsucc (succ 0)) e = id
negation-preserves-parity (negsucc (succ (succ x))) e = negation-preserves-parity (negsucc x) (even-succ-succ (negsucc (succ (succ x))) e)

even-lemma-pos : (x : â„•) â†’ even (pos x) â†’ (pos x /2') â„¤* pos 2 ï¼ pos x
even-lemma-pos 0 even-x = refl
even-lemma-pos (succ 0) even-x = ğŸ˜-elim (even-x â‹†)
even-lemma-pos (succ (succ x)) even-x = succâ„¤ (pos x /2') +â„¤ succâ„¤ (pos x /2')    ï¼âŸ¨ â„¤-left-succ (pos x /2') (succâ„¤ (pos x /2')) âŸ©
                                          succâ„¤ (succâ„¤ ((pos x /2') â„¤* pos 2))       ï¼âŸ¨ ap (Î» z â†’ succâ„¤ (succâ„¤ z)) (even-lemma-pos x even-x) âŸ©
                                          pos (succ (succ x)) âˆ

even-lemma-neg : (x : â„•) â†’ even (negsucc x) â†’ (negsucc x /2') â„¤* pos 2 ï¼ negsucc x
even-lemma-neg x even-x = (âˆ’â„¤ pos (succ x /2)) âˆ’â„¤ pos (succ x /2)  ï¼âŸ¨ negation-dist (pos (succ x /2)) (pos (succ x /2)) âŸ©
                          âˆ’â„¤ (pos (succ x /2) +â„¤ pos (succ x /2)) ï¼âŸ¨ ap âˆ’â„¤_ (even-lemma-pos (succ x) (negation-preserves-parity (negsucc x) even-x)) âŸ©
                          negsucc x âˆ

even-lemma : (x : â„¤) â†’ even x â†’ (x /2') â„¤* pos 2 ï¼ x
even-lemma (pos x) = even-lemma-pos x
even-lemma (negsucc x) = even-lemma-neg x

power-of-pos-positive : âˆ€ n â†’ is-pos-succ (pos (2^ n))
power-of-pos-positive 0 = â‹†
power-of-pos-positive (succ n) = transport is-pos-succ (pos-multiplication-equiv-to-â„• 2 (2^ n)) I
 where
  I : is-pos-succ (pos 2 â„¤* pos (2^ n))
  I = is-pos-succ-mult (pos 2) (pos (2^ n)) â‹† (power-of-pos-positive n)

prod-of-powers : (n a b : â„•) â†’ n â„•^ a â„•* n â„•^ b ï¼ n â„•^ (a +â„• b)
prod-of-powers n a zero     = refl
prod-of-powers n a (succ b) = I
 where
  I : n â„•^ a â„•* n â„•^ succ b ï¼ n â„•^ (a +â„• succ b)
  I = n â„•^ a â„•* n â„•^ succ b   ï¼âŸ¨ refl âŸ©
      n â„•^ a â„•* (n â„•* n â„•^ b) ï¼âŸ¨ mult-associativity (n â„•^ a) n (n â„•^ b) â»Â¹ âŸ©
      n â„•^ a â„•* n â„•* n â„•^ b   ï¼âŸ¨ ap (_â„•* n â„•^ b) (mult-commutativity (n â„•^ a) n) âŸ©
      n â„•* n â„•^ a â„•* n â„•^ b   ï¼âŸ¨ mult-associativity n (n â„•^ a) (n â„•^ b) âŸ©
      n â„•* (n â„•^ a â„•* n â„•^ b) ï¼âŸ¨ ap (n â„•*_) (prod-of-powers n a b) âŸ©
      n â„•* n â„•^ (a +â„• b)       ï¼âŸ¨ refl âŸ©
      n â„•^ succ (a +â„• b)       ï¼âŸ¨ refl âŸ©
      n â„•^ (a +â„• succ b)       âˆ

odd-succ-succ' : (k : â„¤) â†’ odd (succâ„¤ (succâ„¤ k)) â†’ odd k
odd-succ-succ' (pos x) = id
odd-succ-succ' (negsucc zero) = id
odd-succ-succ' (negsucc (succ (succ x))) = id

even-succ-succ' : (k : â„¤) â†’ even (succâ„¤ (succâ„¤ k)) â†’ even k
even-succ-succ' (pos 0) e = id
even-succ-succ' (pos (succ 0)) e = ğŸ˜-elim (e â‹†)
even-succ-succ' (pos (succ (succ x))) e = e
even-succ-succ' (negsucc 0) e = ğŸ˜-elim (e â‹†)
even-succ-succ' (negsucc (succ 0)) e = id
even-succ-succ' (negsucc (succ (succ x))) e = e

times-two-even' : (k : â„¤) â†’ even (k +â„¤ k)
times-two-even' (pos (succ k)) odd2k = times-two-even' (pos k) (odd-succ-succ' (pos k +â„¤ pos k) (transport odd I odd2k))
 where
  I : pos (succ k) +â„¤ pos (succ k) ï¼ pos k +â„¤ pos (succ (succ k))
  I = â„¤-left-succ (pos k) (pos (succ k))
times-two-even' (negsucc (succ k)) odd2k = times-two-even' (negsucc k) (transport odd I (odd-succ-succ (negsucc (succ k) +â„¤ negsucc (succ k)) odd2k))
 where
  I : succâ„¤ (succâ„¤ (negsucc (succ k) +â„¤ negsucc (succ k))) ï¼ negsucc k +â„¤ negsucc k
  I = succâ„¤ (succâ„¤ (negsucc (succ k) +â„¤ negsucc (succ k)))   ï¼âŸ¨ refl âŸ©
      succâ„¤ (succâ„¤ (predâ„¤ (negsucc k) +â„¤ predâ„¤ (negsucc k))) ï¼âŸ¨ refl âŸ©
      succâ„¤ (succâ„¤ (predâ„¤ (predâ„¤ (negsucc k) +â„¤ negsucc k))) ï¼âŸ¨ ap (Î» a â†’ succâ„¤ a) (succpredâ„¤ (predâ„¤ (negsucc k) +â„¤ negsucc k)) âŸ©
      succâ„¤ (predâ„¤ (negsucc k) +â„¤ negsucc k)                 ï¼âŸ¨ ap succâ„¤ (â„¤-left-pred (negsucc k) (negsucc k)) âŸ©
      succâ„¤ (predâ„¤ (negsucc k +â„¤ negsucc k))                 ï¼âŸ¨ succpredâ„¤ (negsucc k +â„¤ negsucc k) âŸ©
      negsucc k +â„¤ negsucc k âˆ

negsucc-lemma : (x : â„•) â†’ negsucc x +â„¤ negsucc x ï¼ negsucc (x +â„• succ x)
negsucc-lemma x = negsucc x +â„¤ negsucc x           ï¼âŸ¨ refl âŸ©
                  (âˆ’â„¤ pos (succ x)) âˆ’â„¤ pos (succ x)  ï¼âŸ¨ negation-dist (pos (succ x)) (pos (succ x)) âŸ©
                  âˆ’â„¤ (pos (succ x) +â„¤ pos (succ x)) ï¼âŸ¨ refl âŸ©
                  âˆ’â„¤ succâ„¤ (pos (succ x) +â„¤ pos x)  ï¼âŸ¨ ap (Î» z â†’ âˆ’â„¤ succâ„¤ z) (distributivity-pos-addition (succ x) x) âŸ©
                  âˆ’â„¤ succâ„¤ (pos (succ x +â„• x))       ï¼âŸ¨ refl âŸ©
                  negsucc (succ x +â„• x)             ï¼âŸ¨ ap negsucc (addition-commutativity (succ x) x) âŸ©
                  negsucc (x +â„• succ x)             âˆ

div-by-two' : (k : â„•) â†’ k +â„• k /2 ï¼ k
div-by-two' 0 = refl
div-by-two' (succ k) = (succ k +â„• succ k) /2     ï¼âŸ¨ ap _/2 (succ-left k (succ k)) âŸ©
                       succ (succ (k +â„• k)) /2  ï¼âŸ¨ refl âŸ©
                       succ ((k +â„• k) /2)        ï¼âŸ¨ ap succ (div-by-two' k) âŸ©
                       succ k                    âˆ

div-by-two : (k : â„¤) â†’ (k +â„¤ k) /2' ï¼ k
div-by-two (pos k) = (pos k +â„¤ pos k) /2' ï¼âŸ¨ ap _/2' (distributivity-pos-addition k k) âŸ©     
                     pos (k +â„• k) /2'      ï¼âŸ¨ ap pos (div-by-two' k) âŸ©
                     pos k âˆ
div-by-two (negsucc x) = (negsucc x +â„¤ negsucc x) /2'   ï¼âŸ¨ ap _/2' (negsucc-lemma x) âŸ©
                         negsucc (x +â„• succ x) /2'     ï¼âŸ¨ refl âŸ©
                         âˆ’â„¤ pos (succ (x +â„• succ x) /2) ï¼âŸ¨ ap (Î» z â†’ âˆ’â„¤ pos (z /2)) (succ-left x (succ x) â»Â¹) âŸ©
                         âˆ’â„¤ pos ((succ x +â„• succ x) /2) ï¼âŸ¨ ap (Î» z â†’ âˆ’â„¤ pos z) (div-by-two' (succ x)) âŸ©
                         negsucc x âˆ

```
